sepcomp/backend/Inliningproof_sepcomp.v
@@ -1,8 +1,20 @@
-Require Import RelationClasses.
-Require Import Classical.
-Require Import Coqlib Coqlib_linker.
+(* *********************************************************************)
+(*                                                                     *)
+(*              The Compcert verified compiler                         *)
+(*                                                                     *)
+(*          Xavier Leroy, INRIA Paris-Rocquencourt                     *)
+(*                                                                     *)
+(*  Copyright Institut National de Recherche en Informatique et en     *)
+(*  Automatique.  All rights reserved.  This file is distributed       *)
+(*  under the terms of the INRIA Non-Commercial License Agreement.     *)
+(*                                                                     *)
+(* *********************************************************************)
+
+(** RTL function inlining: semantic preservation *)
+
+Require Import Coqlib.
 Require Import Errors.
-Require Import Maps Maps_linker.
+Require Import Maps.
 Require Import AST.
 Require Import Integers.
 Require Import Values.
@@ -10,21 +22,15 @@ Require Import Memory.
 Require Import Globalenvs.
 Require Import Events.
 Require Import Smallstep.
-Require Import Language Linker Linkeq.
-Require Import ProgramLSim FunctionLSim.
+Require Import Language.
 Require Import Op.
 Require Import Registers.
 Require Import Inlining.
 Require Import Inliningspec.
 Require Import RTL.
-Require Import Inliningproof.
-Require Import RTL_linker ValueAnalysis_linker.
-Require Import WFType paco.
-
-Set Implicit Arguments.
-
-(** A (compile-time) function environment is compatible with a
-  (run-time) global environment if the following condition holds. *)
+Require Import Maps_sepcomp.
+Require Import Linkeq.
+Require Import SepcompRel.
 
 Lemma funenv_program_spec p i:
   (funenv_program p) ! i =
@@ -75,20 +81,346 @@ Qed.
 
 Section INLINING.
 
-Variable (prog tprog: program).
-Hypothesis TRANSF: transf_program prog = OK tprog.
+Variable prog: program.
+Variable tprog: program.
+Hypothesis TRANSF:
+  @sepcomp_rel
+    Language_RTL Language_RTL
+    (@match_globdef_transf_partial
+       Sig_signature Sig_signature
+       F_RTL F_RTL
+       EF_external_function EF_external_function
+       (Fundef_common F_RTL) (Fundef_common F_RTL)
+       V_unit
+       (fun p f => transf_fundef (funenv_program p) f))
+    prog tprog.
+Let ge := Genv.globalenv prog.
+Let tge := Genv.globalenv tprog.
+Let fenv := funenv_program prog.
 
-Section FUTURE.
+Lemma symbols_preserved:
+  forall (s: ident), Genv.find_symbol tge s = Genv.find_symbol ge s.
+Proof (find_symbol_transf_partial TRANSF).
 
-Variable (fprog ftprog:program).
-Hypothesis (Hfsim: @program_weak_lsim Language_RTL Language_RTL transf_sigT transf_efT transf_vT
-                                      fprog ftprog).
+Lemma varinfo_preserved:
+  forall b, Genv.find_var_info tge b = Genv.find_var_info ge b.
+Proof (find_var_info_transf_partial TRANSF).
 
-Hypothesis (Hfprog: program_linkeq Language_RTL prog fprog).
-Hypothesis (Hftprog: program_linkeq Language_RTL tprog ftprog).
+Lemma functions_translated:
+  forall (v: val) (f: RTL.fundef),
+  Genv.find_funct ge v = Some f ->
+  exists tf, Genv.find_funct tge v = Some tf /\ 
+             exists sprog, program_linkeq Language_RTL sprog prog /\
+                           transf_fundef (funenv_program sprog) f = OK tf.
+Proof (find_funct_transf_partial TRANSF).
 
-Let ge := Genv.globalenv fprog.
-Let tge := Genv.globalenv ftprog.
+Lemma function_ptr_translated:
+  forall (b: block) (f: RTL.fundef),
+  Genv.find_funct_ptr ge b = Some f ->
+  exists tf, Genv.find_funct_ptr tge b = Some tf /\ 
+             exists sprog, program_linkeq Language_RTL sprog prog /\
+                           transf_fundef (funenv_program sprog) f = OK tf.
+Proof (find_funct_ptr_transf_partial TRANSF).
+
+Lemma sig_function_translated:
+  forall fenv f f', transf_fundef fenv f = OK f' -> funsig f' = funsig f.
+Proof.
+  intros. destruct f; Errors.monadInv H.
+  exploit transf_function_spec; eauto. intros SP; inv SP. auto. 
+  auto.
+Qed.
+
+(** ** Properties of contexts and relocations *)
+
+Remark sreg_below_diff:
+  forall ctx r r', Plt r' ctx.(dreg) -> sreg ctx r <> r'.
+Proof.
+  intros. zify. unfold sreg; rewrite shiftpos_eq. xomega. 
+Qed.
+
+Remark context_below_diff:
+  forall ctx1 ctx2 r1 r2,
+  context_below ctx1 ctx2 -> Ple r1 ctx1.(mreg) -> sreg ctx1 r1 <> sreg ctx2 r2.
+Proof.
+  intros. red in H. zify. unfold sreg; rewrite ! shiftpos_eq. xomega.
+Qed.
+
+Remark context_below_lt:
+  forall ctx1 ctx2 r, context_below ctx1 ctx2 -> Ple r ctx1.(mreg) -> Plt (sreg ctx1 r) ctx2.(dreg).
+Proof.
+  intros. red in H. unfold Plt; zify. unfold sreg; rewrite shiftpos_eq. 
+  xomega.
+Qed.
+
+(*
+Remark context_below_le:
+  forall ctx1 ctx2 r, context_below ctx1 ctx2 -> Ple r ctx1.(mreg) -> Ple (sreg ctx1 r) ctx2.(dreg).
+Proof.
+  intros. red in H. unfold Ple; zify. unfold sreg; rewrite shiftpos_eq. 
+  xomega.
+Qed.
+*)
+
+(** ** Agreement between register sets before and after inlining. *)
+
+Definition agree_regs (F: meminj) (ctx: context) (rs rs': regset) :=
+  (forall r, Ple r ctx.(mreg) -> val_inject F rs#r rs'#(sreg ctx r))
+/\(forall r, Plt ctx.(mreg) r -> rs#r = Vundef).
+
+Definition val_reg_charact (F: meminj) (ctx: context) (rs': regset) (v: val) (r: reg) :=
+  (Plt ctx.(mreg) r /\ v = Vundef) \/ (Ple r ctx.(mreg) /\ val_inject F v rs'#(sreg ctx r)).
+
+Remark Plt_Ple_dec:
+  forall p q, {Plt p q} + {Ple q p}.
+Proof.
+  intros. destruct (plt p q). left; auto. right; xomega.
+Qed.
+
+Lemma agree_val_reg_gen:
+  forall F ctx rs rs' r, agree_regs F ctx rs rs' -> val_reg_charact F ctx rs' rs#r r.
+Proof.
+  intros. destruct H as [A B].
+  destruct (Plt_Ple_dec (mreg ctx) r). 
+  left. rewrite B; auto. 
+  right. auto.
+Qed.
+
+Lemma agree_val_regs_gen:
+  forall F ctx rs rs' rl,
+  agree_regs F ctx rs rs' -> list_forall2 (val_reg_charact F ctx rs') rs##rl rl.
+Proof.
+  induction rl; intros; constructor; auto. apply agree_val_reg_gen; auto.
+Qed.
+
+Lemma agree_val_reg:
+  forall F ctx rs rs' r, agree_regs F ctx rs rs' -> val_inject F rs#r rs'#(sreg ctx r).
+Proof.
+  intros. exploit agree_val_reg_gen; eauto. instantiate (1 := r). intros [[A B] | [A B]].
+  rewrite B; auto.
+  auto.
+Qed.
+
+Lemma agree_val_regs:
+  forall F ctx rs rs' rl, agree_regs F ctx rs rs' -> val_list_inject F rs##rl rs'##(sregs ctx rl).
+Proof.
+  induction rl; intros; simpl. constructor. constructor; auto. apply agree_val_reg; auto.
+Qed.
+
+Lemma agree_set_reg:
+  forall F ctx rs rs' r v v',
+  agree_regs F ctx rs rs' ->
+  val_inject F v v' ->
+  Ple r ctx.(mreg) ->
+  agree_regs F ctx (rs#r <- v) (rs'#(sreg ctx r) <- v').
+Proof.
+  unfold agree_regs; intros. destruct H. split; intros.
+  repeat rewrite Regmap.gsspec. 
+  destruct (peq r0 r). subst r0. rewrite peq_true. auto.
+  rewrite peq_false. auto. apply shiftpos_diff; auto. 
+  rewrite Regmap.gso. auto. xomega. 
+Qed.
+
+Lemma agree_set_reg_undef:
+  forall F ctx rs rs' r v',
+  agree_regs F ctx rs rs' ->
+  agree_regs F ctx (rs#r <- Vundef) (rs'#(sreg ctx r) <- v').
+Proof.
+  unfold agree_regs; intros. destruct H. split; intros.
+  repeat rewrite Regmap.gsspec. 
+  destruct (peq r0 r). subst r0. rewrite peq_true. auto.
+  rewrite peq_false. auto. apply shiftpos_diff; auto. 
+  rewrite Regmap.gsspec. destruct (peq r0 r); auto. 
+Qed.
+
+Lemma agree_set_reg_undef':
+  forall F ctx rs rs' r,
+  agree_regs F ctx rs rs' ->
+  agree_regs F ctx (rs#r <- Vundef) rs'.
+Proof.
+  unfold agree_regs; intros. destruct H. split; intros.
+  rewrite Regmap.gsspec. 
+  destruct (peq r0 r). subst r0. auto. auto.
+  rewrite Regmap.gsspec. destruct (peq r0 r); auto. 
+Qed.
+
+Lemma agree_regs_invariant:
+  forall F ctx rs rs1 rs2,
+  agree_regs F ctx rs rs1 ->
+  (forall r, Ple ctx.(dreg) r -> Plt r (ctx.(dreg) + ctx.(mreg)) -> rs2#r = rs1#r) ->
+  agree_regs F ctx rs rs2.
+Proof.
+  unfold agree_regs; intros. destruct H. split; intros.
+  rewrite H0. auto. 
+  apply shiftpos_above.
+  eapply Plt_le_trans. apply shiftpos_below. xomega.
+  apply H1; auto.
+Qed.
+
+Lemma agree_regs_incr:
+  forall F ctx rs1 rs2 F',
+  agree_regs F ctx rs1 rs2 ->
+  inject_incr F F' ->
+  agree_regs F' ctx rs1 rs2.
+Proof.
+  intros. destruct H. split; intros. eauto. auto. 
+Qed.
+
+Remark agree_regs_init:
+  forall F ctx rs, agree_regs F ctx (Regmap.init Vundef) rs.
+Proof.
+  intros; split; intros. rewrite Regmap.gi; auto. rewrite Regmap.gi; auto. 
+Qed.
+
+Lemma agree_regs_init_regs:
+  forall F ctx rl vl vl',
+  val_list_inject F vl vl' ->
+  (forall r, In r rl -> Ple r ctx.(mreg)) ->
+  agree_regs F ctx (init_regs vl rl) (init_regs vl' (sregs ctx rl)).
+Proof.
+  induction rl; simpl; intros.
+  apply agree_regs_init.
+  inv H. apply agree_regs_init.
+  apply agree_set_reg; auto. 
+Qed.
+
+(** ** Executing sequences of moves *)
+
+Lemma tr_moves_init_regs:
+  forall F stk f sp m ctx1 ctx2, context_below ctx1 ctx2 ->
+  forall rdsts rsrcs vl pc1 pc2 rs1,
+  tr_moves f.(fn_code) pc1 (sregs ctx1 rsrcs) (sregs ctx2 rdsts) pc2 ->
+  (forall r, In r rdsts -> Ple r ctx2.(mreg)) ->
+  list_forall2 (val_reg_charact F ctx1 rs1) vl rsrcs ->
+  exists rs2,
+    star step tge (State stk f sp pc1 rs1 m)
+               E0 (State stk f sp pc2 rs2 m)
+  /\ agree_regs F ctx2 (init_regs vl rdsts) rs2
+  /\ forall r, Plt r ctx2.(dreg) -> rs2#r = rs1#r.
+Proof.
+  induction rdsts; simpl; intros.
+(* rdsts = nil *)
+  inv H0. exists rs1; split. apply star_refl. split. apply agree_regs_init. auto.
+(* rdsts = a :: rdsts *)
+  inv H2. inv H0. 
+  exists rs1; split. apply star_refl. split. apply agree_regs_init. auto.
+  simpl in H0. inv H0.
+  exploit IHrdsts; eauto. intros [rs2 [A [B C]]].
+  exists (rs2#(sreg ctx2 a) <- (rs2#(sreg ctx1 b1))).
+  split. eapply star_right. eauto. eapply exec_Iop; eauto. traceEq.
+  split. destruct H3 as [[P Q] | [P Q]].
+  subst a1. eapply agree_set_reg_undef; eauto.
+  eapply agree_set_reg; eauto. rewrite C; auto.  apply context_below_lt; auto.
+  intros. rewrite Regmap.gso. auto. apply sym_not_equal. eapply sreg_below_diff; eauto.
+  destruct H2; discriminate.
+Qed.
+
+(** ** Memory invariants *)
+
+(** A stack location is private if it is not the image of a valid
+   location and we have full rights on it. *)
+
+Definition loc_private (F: meminj) (m m': mem) (sp: block) (ofs: Z) : Prop :=
+  Mem.perm m' sp ofs Cur Freeable /\
+  (forall b delta, F b = Some(sp, delta) -> ~Mem.perm m b (ofs - delta) Max Nonempty).
+
+(** Likewise, for a range of locations. *)
+
+Definition range_private (F: meminj) (m m': mem) (sp: block) (lo hi: Z) : Prop :=
+  forall ofs, lo <= ofs < hi -> loc_private F m m' sp ofs.
+
+Lemma range_private_invariant:
+  forall F m m' sp lo hi F1 m1 m1',
+  range_private F m m' sp lo hi ->
+  (forall b delta ofs,
+      F1 b = Some(sp, delta) ->
+      Mem.perm m1 b ofs Max Nonempty ->
+      lo <= ofs + delta < hi ->
+      F b = Some(sp, delta) /\ Mem.perm m b ofs Max Nonempty) ->
+  (forall ofs, Mem.perm m' sp ofs Cur Freeable -> Mem.perm m1' sp ofs Cur Freeable) ->
+  range_private F1 m1 m1' sp lo hi.
+Proof.
+  intros; red; intros. exploit H; eauto. intros [A B]. split; auto.
+  intros; red; intros. exploit H0; eauto. omega. intros [P Q]. 
+  eelim B; eauto.
+Qed.
+
+Lemma range_private_perms:
+  forall F m m' sp lo hi,
+  range_private F m m' sp lo hi ->
+  Mem.range_perm m' sp lo hi Cur Freeable.
+Proof.
+  intros; red; intros. eapply H; eauto.
+Qed.
+
+Lemma range_private_alloc_left:
+  forall F m m' sp' base hi sz m1 sp F1,
+  range_private F m m' sp' base hi ->
+  Mem.alloc m 0 sz = (m1, sp) ->
+  F1 sp = Some(sp', base) ->
+  (forall b, b <> sp -> F1 b = F b) ->
+  range_private F1 m1 m' sp' (base + Zmax sz 0) hi.
+Proof.
+  intros; red; intros. 
+  exploit (H ofs). generalize (Zmax2 sz 0). omega. intros [A B].
+  split; auto. intros; red; intros.
+  exploit Mem.perm_alloc_inv; eauto.
+  destruct (eq_block b sp); intros.
+  subst b. rewrite H1 in H4; inv H4. 
+  rewrite Zmax_spec in H3. destruct (zlt 0 sz); omega.
+  rewrite H2 in H4; auto. eelim B; eauto. 
+Qed.
+
+Lemma range_private_free_left:
+  forall F m m' sp base sz hi b m1,
+  range_private F m m' sp (base + Zmax sz 0) hi ->
+  Mem.free m b 0 sz = Some m1 ->
+  F b = Some(sp, base) ->
+  Mem.inject F m m' ->
+  range_private F m1 m' sp base hi.
+Proof.
+  intros; red; intros. 
+  destruct (zlt ofs (base + Zmax sz 0)) as [z|z].
+  red; split. 
+  replace ofs with ((ofs - base) + base) by omega.
+  eapply Mem.perm_inject; eauto.
+  eapply Mem.free_range_perm; eauto.
+  rewrite Zmax_spec in z. destruct (zlt 0 sz); omega. 
+  intros; red; intros. destruct (eq_block b b0).
+  subst b0. rewrite H1 in H4; inv H4.
+  eelim Mem.perm_free_2; eauto. rewrite Zmax_spec in z. destruct (zlt 0 sz); omega.
+  exploit Mem.mi_no_overlap; eauto. 
+  apply Mem.perm_cur_max. apply Mem.perm_implies with Freeable; auto with mem.
+  eapply Mem.free_range_perm. eauto. 
+  instantiate (1 := ofs - base). rewrite Zmax_spec in z. destruct (zlt 0 sz); omega.
+  eapply Mem.perm_free_3; eauto. 
+  intros [A | A]. congruence. omega. 
+
+  exploit (H ofs). omega. intros [A B]. split. auto.
+  intros; red; intros. eelim B; eauto. eapply Mem.perm_free_3; eauto.
+Qed.
+
+Lemma range_private_extcall:
+  forall F F' m1 m2 m1' m2' sp base hi,
+  range_private F m1 m1' sp base hi ->
+  (forall b ofs p,
+     Mem.valid_block m1 b -> Mem.perm m2 b ofs Max p -> Mem.perm m1 b ofs Max p) ->
+  Mem.unchanged_on (loc_out_of_reach F m1) m1' m2' ->
+  Mem.inject F m1 m1' ->
+  inject_incr F F' ->
+  inject_separated F F' m1 m1' ->
+  Mem.valid_block m1' sp ->
+  range_private F' m2 m2' sp base hi.
+Proof.
+  intros until hi; intros RP PERM UNCH INJ INCR SEP VB.
+  red; intros. exploit RP; eauto. intros [A B].
+  split. eapply Mem.perm_unchanged_on; eauto. 
+  intros. red in SEP. destruct (F b) as [[sp1 delta1] |] eqn:?.
+  exploit INCR; eauto. intros EQ; rewrite H0 in EQ; inv EQ. 
+  red; intros; eelim B; eauto. eapply PERM; eauto. 
+  red. destruct (plt b (Mem.nextblock m1)); auto. 
+  exploit Mem.mi_freeblocks; eauto. congruence.
+  exploit SEP; eauto. tauto. 
+Qed.
 
 (** ** Relating global environments *)
 
@@ -106,8 +438,10 @@ Lemma find_function_agree:
   agree_regs F ctx rs rs' ->
   match_globalenvs F bound ->
   exists fd',
-  find_function tge (sros ctx ros) rs' = Some fd' /\
-  globfun_weak_lsim Language_RTL Language_RTL transf_sigT transf_efT ge tge fd fd'.
+  find_function tge (sros ctx ros) rs' = Some fd' /\ 
+  exists sprog,
+    program_linkeq Language_RTL sprog prog /\
+    transf_fundef (funenv_program sprog) fd = OK fd'.
 Proof.
   intros. destruct ros as [r | id]; simpl in *.
   (* register *)
@@ -120,8 +454,8 @@ Proof.
     rewrite EQ in H; rewrite Genv.find_funct_find_funct_ptr in H. auto.
   rewrite H2. eapply functions_translated; eauto.
   (* symbol *)
-  unfold ge, tge in *. erewrite symbols_preserved; try apply Hfsim. destruct (Genv.find_symbol (Genv.globalenv fprog) id); try discriminate.
-  eapply funct_ptr_translated; eauto.
+  rewrite symbols_preserved. destruct (Genv.find_symbol ge id); try discriminate.
+  eapply function_ptr_translated; eauto.
 Qed.
 
 (** ** Relating stacks *)
@@ -132,10 +466,10 @@ Inductive match_stacks (F: meminj) (m m': mem):
         (MG: match_globalenvs F bound1)
         (BELOW: Ple bound1 bound),
       match_stacks F m m' nil nil bound
-  | match_stacks_cons: forall res f sp pc rs stk f' sp' rs' stk' bound ctx fenv
+  | match_stacks_cons: forall res f sp pc rs stk f' sp' rs' stk' bound ctx sprog
+        (SPROG: program_linkeq Language_RTL sprog prog)
         (MS: match_stacks_inside F m m' stk stk' f' ctx sp' rs')
-        (FENV: PTree_le fenv (funenv_program fprog))
-        (FB: tr_funbody fenv f'.(fn_stacksize) ctx f f'.(fn_code))
+        (FB: tr_funbody (funenv_program sprog) f'.(fn_stacksize) ctx f f'.(fn_code))
         (AG: agree_regs F ctx rs rs')
         (SP: F sp = Some(sp', ctx.(dstk)))
         (PRIV: range_private F m m' sp' (ctx.(dstk) + ctx.(mstk)) f'.(fn_stacksize))
@@ -166,10 +500,10 @@ with match_stacks_inside (F: meminj) (m m': mem):
         (RET: ctx.(retinfo) = None)
         (DSTK: ctx.(dstk) = 0),
       match_stacks_inside F m m' stk stk' f' ctx sp' rs'
-  | match_stacks_inside_inlined: forall res f sp pc rs stk stk' f' ctx sp' rs' ctx' fenv
+  | match_stacks_inside_inlined: forall res f sp pc rs stk stk' f' ctx sp' rs' ctx' sprog
+        (SPROG: program_linkeq Language_RTL sprog prog)
         (MS: match_stacks_inside F m m' stk stk' f' ctx' sp' rs')
-        (FENV: PTree_le fenv (funenv_program fprog))
-        (FB: tr_funbody fenv f'.(fn_stacksize) ctx' f f'.(fn_code))
+        (FB: tr_funbody (funenv_program sprog) f'.(fn_stacksize) ctx' f f'.(fn_code))
         (AG: agree_regs F ctx' rs rs')
         (SP: F sp = Some(sp', ctx'.(dstk)))
         (PAD: range_private F m m' sp' (ctx'.(dstk) + ctx'.(mstk)) ctx.(dstk))
@@ -266,7 +600,7 @@ Proof.
   intros. apply IMAGE with delta. eapply INJ; eauto. eapply Plt_le_trans; eauto.
   auto. auto.
   (* cons *)
-  apply match_stacks_cons with (ctx := ctx) (fenv := fenv); auto.
+  apply match_stacks_cons with (ctx := ctx) (sprog := sprog); auto.
   eapply match_stacks_inside_invariant; eauto.
   intros; eapply INJ; eauto; xomega. 
   intros; eapply PERM1; eauto; xomega.
@@ -292,7 +626,7 @@ Proof.
   intros; eapply PERM2; eauto; xomega.
   intros; eapply PERM3; eauto; xomega.
   (* inlined *)
-  apply match_stacks_inside_inlined with (ctx' := ctx') (fenv := fenv); auto. 
+  apply match_stacks_inside_inlined with (ctx' := ctx') (sprog := sprog); auto. 
   apply IHmatch_stacks_inside; auto.
   intros. apply RS. red in BELOW. xomega. 
   apply agree_regs_incr with F; auto. 
@@ -485,23 +819,24 @@ Proof.
 Qed.
 
 Lemma match_stacks_inside_inlined_tailcall:
-  forall F m m' stk stk' f' ctx sp' rs' ctx' f fenv,
+  forall F m m' stk stk' f' ctx sp' rs' ctx' f sprog,
+  program_linkeq Language_RTL sprog prog ->
   match_stacks_inside F m m' stk stk' f' ctx sp' rs' ->
   context_below ctx ctx' ->
   context_stack_tailcall ctx f ctx' ->
   ctx'.(retinfo) = ctx.(retinfo) ->
   range_private F m m' sp' ctx.(dstk) f'.(fn_stacksize) ->
-  tr_funbody fenv f'.(fn_stacksize) ctx' f f'.(fn_code) ->
+  tr_funbody (funenv_program sprog) f'.(fn_stacksize) ctx' f f'.(fn_code) ->
   match_stacks_inside F m m' stk stk' f' ctx' sp' rs'.
 Proof.
-  intros. inv H.
+  intros. inv H0.
   (* base *)
   eapply match_stacks_inside_base; eauto. congruence. 
-  rewrite H1. rewrite DSTK. apply align_unchanged. apply min_alignment_pos. apply Zdivide_0.
+  rewrite H2. rewrite DSTK. apply align_unchanged. apply min_alignment_pos. apply Zdivide_0.
   (* inlined *)
-  assert (dstk ctx <= dstk ctx'). rewrite H1. apply align_le. apply min_alignment_pos.
+  assert (dstk ctx <= dstk ctx'). rewrite H2. apply align_le. apply min_alignment_pos.
   eapply match_stacks_inside_inlined; eauto. 
-  red; intros. destruct (zlt ofs (dstk ctx)). apply PAD; omega. apply H3. inv H4. xomega. 
+  red; intros. destruct (zlt ofs (dstk ctx)). apply PAD; omega. apply H4. inv H5. xomega. 
   congruence. 
   unfold context_below in *. xomega.
   unfold context_stack_call in *. omega. 
@@ -509,11 +844,11 @@ Qed.
 
 (** ** Relating states *)
 
-Inductive match_states (F:meminj): state -> state -> Prop :=
-  | match_regular_states: forall stk f sp pc rs m stk' f' sp' rs' m' ctx fenv
+Inductive match_states: state -> state -> Prop :=
+  | match_regular_states: forall stk f sp pc rs m stk' f' sp' rs' m' F ctx sprog
+        (SPROG: program_linkeq Language_RTL sprog prog)
         (MS: match_stacks_inside F m m' stk stk' f' ctx sp' rs')
-        (FENV: PTree_le fenv (funenv_program fprog))
-        (FB: tr_funbody fenv f'.(fn_stacksize) ctx f f'.(fn_code))
+        (FB: tr_funbody (funenv_program sprog) f'.(fn_stacksize) ctx f f'.(fn_code))
         (AG: agree_regs F ctx rs rs')
         (SP: F sp = Some(sp', ctx.(dstk)))
         (MINJ: Mem.inject F m m')
@@ -521,13 +856,20 @@ Inductive match_states (F:meminj): state -> state -> Prop :=
         (PRIV: range_private F m m' sp' (ctx.(dstk) + ctx.(mstk)) f'.(fn_stacksize))
         (SSZ1: 0 <= f'.(fn_stacksize) < Int.max_unsigned)
         (SSZ2: forall ofs, Mem.perm m' sp' ofs Max Nonempty -> 0 <= ofs <= f'.(fn_stacksize)),
-      match_states F
-                   (State stk f (Vptr sp Int.zero) pc rs m)
+      match_states (State stk f (Vptr sp Int.zero) pc rs m)
                    (State stk' f' (Vptr sp' Int.zero) (spc ctx pc) rs' m')
-  | match_call_regular_states: forall stk f vargs m stk' f' sp' rs' m' ctx ctx' pc' pc1' rargs fenv
+  | match_call_states: forall stk fd args m stk' fd' args' m' F sprog
+        (SPROG: program_linkeq Language_RTL sprog prog)
+        (MS: match_stacks F m m' stk stk' (Mem.nextblock m'))
+        (FD: transf_fundef (funenv_program sprog) fd = OK fd')
+        (VINJ: val_list_inject F args args')
+        (MINJ: Mem.inject F m m'),
+      match_states (Callstate stk fd args m)
+                   (Callstate stk' fd' args' m')
+  | match_call_regular_states: forall stk f vargs m stk' f' sp' rs' m' F ctx ctx' pc' pc1' rargs sprog
+        (SPROG: program_linkeq Language_RTL sprog prog)
         (MS: match_stacks_inside F m m' stk stk' f' ctx sp' rs')
-        (FENV: PTree_le fenv (funenv_program fprog))
-        (FB: tr_funbody fenv f'.(fn_stacksize) ctx f f'.(fn_code))
+        (FB: tr_funbody (funenv_program sprog) f'.(fn_stacksize) ctx f f'.(fn_code))
         (BELOW: context_below ctx' ctx)
         (NOP: f'.(fn_code)!pc' = Some(Inop pc1'))
         (MOVES: tr_moves f'.(fn_code) pc1' (sregs ctx' rargs) (sregs ctx f.(fn_params)) (spc ctx f.(fn_entrypoint)))
@@ -537,17 +879,15 @@ Inductive match_states (F:meminj): state -> state -> Prop :=
         (PRIV: range_private F m m' sp' ctx.(dstk) f'.(fn_stacksize))
         (SSZ1: 0 <= f'.(fn_stacksize) < Int.max_unsigned)
         (SSZ2: forall ofs, Mem.perm m' sp' ofs Max Nonempty -> 0 <= ofs <= f'.(fn_stacksize)),
-      match_states F
-                   (Callstate stk (Internal f) vargs m)
+      match_states (Callstate stk (Internal f) vargs m)
                    (State stk' f' (Vptr sp' Int.zero) pc' rs' m')
-  | match_return_states: forall stk v m stk' v' m'
+  | match_return_states: forall stk v m stk' v' m' F
         (MS: match_stacks F m m' stk stk' (Mem.nextblock m'))
         (VINJ: val_inject F v v')
         (MINJ: Mem.inject F m m'),
-      match_states F
-                   (Returnstate stk v m)
+      match_states (Returnstate stk v m)
                    (Returnstate stk' v' m')
-  | match_return_regular_states: forall stk v m stk' f' sp' rs' m' ctx pc' or rinfo
+  | match_return_regular_states: forall stk v m stk' f' sp' rs' m' F ctx pc' or rinfo
         (MS: match_stacks_inside F m m' stk stk' f' ctx sp' rs')
         (RET: ctx.(retinfo) = Some rinfo)
         (AT: f'.(fn_code)!pc' = Some(inline_return ctx or rinfo))
@@ -557,20 +897,8 @@ Inductive match_states (F:meminj): state -> state -> Prop :=
         (PRIV: range_private F m m' sp' ctx.(dstk) f'.(fn_stacksize))
         (SSZ1: 0 <= f'.(fn_stacksize) < Int.max_unsigned)
         (SSZ2: forall ofs, Mem.perm m' sp' ofs Max Nonempty -> 0 <= ofs <= f'.(fn_stacksize)),
-      match_states F
-                   (Returnstate stk v m)
+      match_states (Returnstate stk v m)
                    (State stk' f' (Vptr sp' Int.zero) pc' rs' m').
-
-Inductive match_call (F:meminj): state -> state -> Prop :=
-  | match_call_states: forall stk fd args m stk' fd' args' m'
-        (MS: match_stacks F m m' stk stk' (Mem.nextblock m'))
-        (FD: globfun_weak_lsim Language_RTL Language_RTL transf_sigT transf_efT ge tge fd fd')
-        (VINJ: val_list_inject F args args')
-        (MINJ: Mem.inject F m m'),
-      match_call F
-                 (Callstate stk fd args m)
-                 (Callstate stk' fd' args' m')
-.
 
 (** ** Forward simulation *)
 
@@ -582,26 +910,26 @@ Definition measure (S: state) : nat :=
   end.
 
 Lemma tr_funbody_inv:
-  forall sz cts f c pc i fenv,
+  forall fenv sz cts f c pc i,
   tr_funbody fenv sz cts f c -> f.(fn_code)!pc = Some i -> tr_instr fenv sz cts pc i c.
 Proof.
   intros. inv H. eauto. 
 Qed.
 
 Theorem step_simulation:
-  forall F S1 t S2,
+  forall S1 t S2,
   step ge S1 t S2 ->
-  forall S1' (MS: match_states F S1 S1'),
-  (exists F' S2', plus step tge S1' t S2' /\ (match_states F' S2 S2' \/ match_call F' S2 S2'))
-  \/ (exists F', measure S2 < measure S1 /\ t = E0 /\ (match_states F' S2 S1' \/ match_call F' S2 S1'))%nat.
+  forall S1' (MS: match_states S1 S1'),
+  (exists S2', plus step tge S1' t S2' /\ match_states S2 S2')
+  \/ (measure S2 < measure S1 /\ t = E0 /\ match_states S2 S1')%nat.
 Proof.
   induction 1; intros; inv MS.
 
 (* nop *)
   exploit tr_funbody_inv; eauto. intros TR; inv TR.
-  left; econstructor; econstructor; split. 
+  left; econstructor; split. 
   eapply plus_one. eapply exec_Inop; eauto.
-  left. econstructor; eauto.
+  econstructor; eauto.
 
 (* op *)
   exploit tr_funbody_inv; eauto. intros TR; inv TR.
@@ -611,10 +939,10 @@ Proof.
     instantiate (2 := rs##args). instantiate (1 := rs'##(sregs ctx args)). eapply agree_val_regs; eauto.
     eexact MINJ. eauto.
   fold (sop ctx op). intros [v' [A B]].
-  left; econstructor; econstructor; split.
+  left; econstructor; split.
   eapply plus_one. eapply exec_Iop; eauto. erewrite eval_operation_preserved; eauto.
-  apply symbols_preserved. auto.
-  left. econstructor; eauto. 
+  exact symbols_preserved. 
+  econstructor; eauto. 
   apply match_stacks_inside_set_reg; auto.
   apply agree_set_reg; auto. 
   
@@ -628,10 +956,10 @@ Proof.
   fold (saddr ctx addr). intros [a' [P Q]].
   exploit Mem.loadv_inject; eauto. intros [v' [U V]].
   assert (eval_addressing tge (Vptr sp' Int.zero) (saddr ctx addr) rs' ## (sregs ctx args) = Some a').
-  rewrite <- P. apply eval_addressing_preserved. apply symbols_preserved. auto.
-  left; econstructor; econstructor; split.
+  rewrite <- P. apply eval_addressing_preserved. exact symbols_preserved.
+  left; econstructor; split.
   eapply plus_one. eapply exec_Iload; eauto.
-  left. econstructor; eauto. 
+  econstructor; eauto. 
   apply match_stacks_inside_set_reg; auto.
   apply agree_set_reg; auto. 
 
@@ -646,12 +974,12 @@ Proof.
   exploit Mem.storev_mapped_inject; eauto. eapply agree_val_reg; eauto. 
   intros [m1' [U V]].
   assert (eval_addressing tge (Vptr sp' Int.zero) (saddr ctx addr) rs' ## (sregs ctx args) = Some a').
-    rewrite <- P. apply eval_addressing_preserved. apply symbols_preserved. auto.
-  left; econstructor; econstructor; split.
+    rewrite <- P. apply eval_addressing_preserved. exact symbols_preserved.
+  left; econstructor; split.
   eapply plus_one. eapply exec_Istore; eauto.
   destruct a; simpl in H1; try discriminate.
   destruct a'; simpl in U; try discriminate.
-  left. econstructor; eauto.
+  econstructor; eauto.
   eapply match_stacks_inside_store; eauto.
   eapply Mem.store_valid_block_1; eauto.
   eapply range_private_invariant; eauto.
@@ -661,31 +989,31 @@ Proof.
 
 (* call *)
   exploit match_stacks_inside_globalenvs; eauto. intros [bound G].
-  exploit find_function_agree; eauto. intros [fd' [A B]].
+  exploit find_function_agree; eauto. intros [fd' [A [sprog' [Hsprog' B]]]].
   exploit tr_funbody_inv; eauto. intros TR; inv TR.
 (* not inlined *)
-  left; econstructor; econstructor; split.
+  left; econstructor; split.
   eapply plus_one. eapply exec_Icall; eauto.
-  eapply sig_preserved; eauto.
-  right. econstructor; eauto.
-  eapply match_stacks_cons; eauto. 
+  eapply sig_function_translated; eauto.
+  econstructor; eauto.
+  eapply match_stacks_cons; try apply FB; eauto. 
   eapply agree_val_regs; eauto. 
 (* inlined *)
   assert (fd = Internal f0).
     simpl in H0. destruct (Genv.find_symbol ge id) as [b|] eqn:?; try discriminate.
-    exploit funenv_program_compat; eauto. apply FENV. eauto. intros.
+    exploit (funenv_program_compat prog); eauto. destruct (program_linkeq_fenv_le _ _ SPROG). apply H1. eauto. intros. 
     unfold ge in H0. congruence.
   subst fd.
-  right; econstructor; split. simpl; omega. split. auto. 
-  left. econstructor; eauto. 
-  eapply match_stacks_inside_inlined; eauto.
+  right; split. simpl; omega. split. auto. 
+  econstructor; try apply H13; eauto. 
+  eapply match_stacks_inside_inlined; try apply FB; eauto.
   red; intros. apply PRIV. inv H13. destruct H16. xomega.
   apply agree_val_regs_gen; auto.
   red; intros; apply PRIV. destruct H16. omega. 
 
 (* tailcall *)
   exploit match_stacks_inside_globalenvs; eauto. intros [bound G].
-  exploit find_function_agree; eauto. intros [fd' [A B]].
+  exploit find_function_agree; eauto. intros [fd' [A [sprog' [Hsprog' B]]]].
   assert (PRIV': range_private F m' m'0 sp' (dstk ctx) f'.(fn_stacksize)).
     eapply range_private_free_left; eauto. inv FB. rewrite <- H4. auto. 
   exploit tr_funbody_inv; eauto. intros TR; inv TR.
@@ -698,10 +1026,10 @@ Proof.
     eapply Mem.free_range_perm; eauto. omega.
     inv FB. eapply range_private_perms; eauto. xomega.
   destruct X as [m1' FREE].
-  left; econstructor; econstructor; split.
+  left; econstructor; split.
   eapply plus_one. eapply exec_Itailcall; eauto.
-  eapply sig_preserved; eauto.
-  right. econstructor; eauto.
+  eapply sig_function_translated; eauto.
+  econstructor; eauto.
   eapply match_stacks_bound with (bound := sp'). 
   eapply match_stacks_invariant; eauto.
     intros. eapply Mem.perm_free_3; eauto. 
@@ -715,10 +1043,10 @@ Proof.
   eelim Q; eauto. replace (ofs + delta - delta) with ofs by omega. 
   apply Mem.perm_max with k. apply Mem.perm_implies with p; auto with mem.
 (* turned into a call *)
-  left; econstructor; econstructor; split.
+  left; econstructor; split.
   eapply plus_one. eapply exec_Icall; eauto.
-  eapply sig_preserved; eauto.
-  right. econstructor; eauto.
+  eapply sig_function_translated; eauto.
+  econstructor; eauto.
   eapply match_stacks_untailcall; eauto.
   eapply match_stacks_inside_invariant; eauto. 
     intros. eapply Mem.perm_free_3; eauto.
@@ -727,12 +1055,12 @@ Proof.
 (* inlined *)
   assert (fd = Internal f0).
     simpl in H0. destruct (Genv.find_symbol ge id) as [b|] eqn:?; try discriminate.
-    exploit funenv_program_compat; eauto. apply FENV. eauto. intros.
+    exploit (funenv_program_compat prog); eauto. destruct (program_linkeq_fenv_le _ _ SPROG). apply H1. eauto. intros. 
     unfold ge in H0. congruence.
   subst fd.
-  right; econstructor; split. simpl; omega. split. auto. 
-  left. econstructor; eauto.
-  eapply match_stacks_inside_inlined_tailcall; eauto.
+  right; split. simpl; omega. split. auto. 
+  econstructor; try apply H8; eauto.
+  eapply match_stacks_inside_inlined_tailcall; try apply H8; eauto.
   eapply match_stacks_inside_invariant; eauto.
     intros. eapply Mem.perm_free_3; eauto.
   apply agree_val_regs_gen; auto.
@@ -747,16 +1075,17 @@ Proof.
     eapply match_stacks_inside_globals; eauto.
     instantiate (1 := rs'##(sregs ctx args)). eapply agree_val_regs; eauto. 
   intros [F1 [v1 [m1' [A [B [C [D [E [J K]]]]]]]]].
-  left; econstructor; econstructor; split.
+  left; econstructor; split.
   eapply plus_one. eapply exec_Ibuiltin; eauto. 
     eapply external_call_symbols_preserved; eauto. 
-    apply symbols_preserved. auto. apply varinfo_preserved. auto.
-  left. econstructor.
+    exact symbols_preserved. exact varinfo_preserved.
+  econstructor.
+    eauto.
     eapply match_stacks_inside_set_reg. 
     eapply match_stacks_inside_extcall with (F1 := F) (F2 := F1) (m1 := m) (m1' := m'0); eauto.
     intros; eapply external_call_max_perm; eauto. 
     intros; eapply external_call_max_perm; eauto. 
-  auto. eauto. auto.
+  auto. 
   eapply agree_set_reg. eapply agree_regs_incr; eauto. auto. auto. 
   apply J; auto.
   auto. 
@@ -770,18 +1099,18 @@ Proof.
   exploit tr_funbody_inv; eauto. intros TR; inv TR.
   assert (eval_condition cond rs'##(sregs ctx args) m' = Some b).
     eapply eval_condition_inject; eauto. eapply agree_val_regs; eauto. 
-  left; econstructor; econstructor; split.
+  left; econstructor; split.
   eapply plus_one. eapply exec_Icond; eauto. 
-  destruct b; left; econstructor; eauto. 
+  destruct b; econstructor; eauto. 
 
 (* jumptable *)
   exploit tr_funbody_inv; eauto. intros TR; inv TR.
   assert (val_inject F rs#arg rs'#(sreg ctx arg)). eapply agree_val_reg; eauto.
   rewrite H0 in H2; inv H2. 
-  left; econstructor; econstructor; split.
+  left; econstructor; split.
   eapply plus_one. eapply exec_Ijumptable; eauto.
   rewrite list_nth_z_map. rewrite H1. simpl; reflexivity. 
-  left. econstructor; eauto. 
+  econstructor; eauto. 
 
 (* return *)
   exploit tr_funbody_inv; eauto. intros TR; inv TR.
@@ -795,9 +1124,9 @@ Proof.
     inv FB. eapply range_private_perms; eauto.
     generalize (Zmax_spec (fn_stacksize f) 0). destruct (zlt 0 (fn_stacksize f)); omega.
   destruct X as [m1' FREE].
-  left; econstructor; econstructor; split.
+  left; econstructor; split.
   eapply plus_one. eapply exec_Ireturn; eauto. 
-  left. econstructor; eauto.
+  econstructor; eauto.
   eapply match_stacks_bound with (bound := sp'). 
   eapply match_stacks_invariant; eauto.
     intros. eapply Mem.perm_free_3; eauto. 
@@ -815,13 +1144,48 @@ Proof.
   apply Mem.perm_max with k. apply Mem.perm_implies with p; auto with mem.
 
   (* inlined *)
-  right. econstructor. split. simpl. omega. split. auto. 
-  left. econstructor; eauto.
+  right. split. simpl. omega. split. auto. 
+  econstructor; eauto.
   eapply match_stacks_inside_invariant; eauto. 
     intros. eapply Mem.perm_free_3; eauto.
   destruct or; simpl. apply agree_val_reg; auto. auto.
   eapply Mem.free_left_inject; eauto.
   inv FB. rewrite H4 in PRIV. eapply range_private_free_left; eauto. 
+
+(* internal function, not inlined *)
+  assert (A: exists f', tr_function (funenv_program sprog) f f' /\ fd' = Internal f'). 
+    Errors.monadInv FD. exists x. split; auto. eapply transf_function_spec; eauto. 
+  destruct A as [f' [TR EQ]]. inversion TR; subst.
+  exploit Mem.alloc_parallel_inject. eauto. eauto. apply Zle_refl. 
+    instantiate (1 := fn_stacksize f'). inv H0. xomega. 
+  intros [F' [m1' [sp' [A [B [C [D E]]]]]]].
+  left; econstructor; split.
+  eapply plus_one. eapply exec_function_internal; eauto.
+  rewrite H5. econstructor. eauto.
+  instantiate (1 := F'). apply match_stacks_inside_base.
+  assert (SP: sp' = Mem.nextblock m'0) by (eapply Mem.alloc_result; eauto).
+  rewrite <- SP in MS0. 
+  eapply match_stacks_invariant; eauto.
+    intros. destruct (eq_block b1 stk). 
+    subst b1. rewrite D in H7; inv H7. subst b2. eelim Plt_strict; eauto.  
+    rewrite E in H7; auto. 
+    intros. exploit Mem.perm_alloc_inv. eexact H. eauto. 
+    destruct (eq_block b1 stk); intros; auto. 
+    subst b1. rewrite D in H7; inv H7. subst b2. eelim Plt_strict; eauto.  
+    intros. eapply Mem.perm_alloc_1; eauto. 
+    intros. exploit Mem.perm_alloc_inv. eexact A. eauto. 
+    rewrite dec_eq_false; auto.
+  auto. auto. auto. 
+  rewrite H4. apply agree_regs_init_regs. eauto. auto. inv H0; auto. congruence. auto.
+  eapply Mem.valid_new_block; eauto.
+  red; intros. split.
+  eapply Mem.perm_alloc_2; eauto. inv H0; xomega.
+  intros; red; intros. exploit Mem.perm_alloc_inv. eexact H. eauto.
+  destruct (eq_block b stk); intros. 
+  subst. rewrite D in H8; inv H8. inv H0; xomega.
+  rewrite E in H8; auto. eelim Mem.fresh_block_alloc. eexact A. eapply Mem.mi_mappedblocks; eauto.
+  auto.
+  intros. exploit Mem.perm_alloc_inv; eauto. rewrite dec_eq_true. omega. 
 
 (* internal function, inlined *)
   inversion FB; subst.
@@ -847,24 +1211,43 @@ Proof.
     apply Mem.perm_max with k. apply Mem.perm_implies with p; auto with mem.
   intros [F' [A [B [C D]]]].
   exploit tr_moves_init_regs; eauto. intros [rs'' [P [Q R]]].
-  left; econstructor; econstructor; split. 
+  left; econstructor; split. 
   eapply plus_left. eapply exec_Inop; eauto. eexact P. traceEq.
-  left. econstructor.
+  econstructor. eauto.
   eapply match_stacks_inside_alloc_left; eauto.
   eapply match_stacks_inside_invariant; eauto.
   omega.
-  eauto. auto.
+  auto.
   apply agree_regs_incr with F; auto.
   auto. auto. auto.
   rewrite H2. eapply range_private_alloc_left; eauto.
   auto. auto.
 
+(* external function *)
+  exploit match_stacks_globalenvs; eauto. intros [bound MG].
+  exploit external_call_mem_inject; eauto. 
+    eapply match_globalenvs_preserves_globals; eauto.
+  intros [F1 [v1 [m1' [A [B [C [D [E [J K]]]]]]]]].
+  simpl in FD. inv FD. 
+  left; econstructor; split.
+  eapply plus_one. eapply exec_function_external; eauto. 
+    eapply external_call_symbols_preserved; eauto. 
+    exact symbols_preserved. exact varinfo_preserved.
+  econstructor.
+    eapply match_stacks_bound with (Mem.nextblock m'0).
+    eapply match_stacks_extcall with (F1 := F) (F2 := F1) (m1 := m) (m1' := m'0); eauto.
+    intros; eapply external_call_max_perm; eauto. 
+    intros; eapply external_call_max_perm; eauto.
+    xomega.
+    eapply external_call_nextblock; eauto. 
+    auto. auto.
+
 (* return fron noninlined function *)
   inv MS0.
   (* normal case *)
-  left; econstructor; econstructor; split.
+  left; econstructor; split.
   eapply plus_one. eapply exec_return.
-  left. econstructor; eauto. 
+  econstructor; eauto. 
   apply match_stacks_inside_set_reg; auto. 
   apply agree_set_reg; auto.
   (* untailcall case *)
@@ -875,11 +1258,11 @@ Proof.
   assert (res0 = res). unfold sreg in H1; unfold reg in *; xomega.
   subst rpc res0.
 *)
-  left; econstructor; econstructor; split.
+  left; econstructor; split.
   eapply plus_one. eapply exec_return.
-  left. eapply match_regular_states. 
+  eapply match_regular_states. eauto. 
   eapply match_stacks_inside_set_reg; eauto.
-  eauto. auto. 
+  auto. 
   apply agree_set_reg; auto.
   auto. auto. auto.
   red; intros. destruct (zlt ofs (dstk ctx)). apply PAD; omega. apply PRIV; omega.
@@ -892,26 +1275,26 @@ Proof.
     red; intros. destruct (zlt ofs (dstk ctx)). apply PAD. omega. apply PRIV. omega.
   destruct or.
   (* with a result *)
-  left; econstructor; econstructor; split. 
+  left; econstructor; split. 
   eapply plus_one. eapply exec_Iop; eauto. simpl. reflexivity. 
-  left. econstructor; eauto. apply match_stacks_inside_set_reg; auto. apply agree_set_reg; auto.
+  econstructor; eauto. apply match_stacks_inside_set_reg; auto. apply agree_set_reg; auto.
   (* without a result *)
-  left; econstructor; econstructor; split. 
+  left; econstructor; split. 
   eapply plus_one. eapply exec_Inop; eauto.
-  left. econstructor; eauto. subst vres. apply agree_set_reg_undef'; auto.
+  econstructor; eauto. subst vres. apply agree_set_reg_undef'; auto.
 Qed.
 
 Lemma transf_initial_states:
-  forall st1, initial_state fprog st1 -> exists F st2, initial_state ftprog st2 /\ match_call F st1 st2.
+  forall st1, initial_state prog st1 -> exists st2, initial_state tprog st2 /\ match_states st1 st2.
 Proof.
   intros. inv H.
-  exploit funct_ptr_translated; eauto. intros [tf [FIND TR]].
-  eexists. exists (Callstate nil tf nil m0); split.
+  exploit function_ptr_translated; eauto. intros [tf [FIND [sprog [Hsprog TR]]]].
+  exists (Callstate nil tf nil m0); split.
   econstructor; eauto.
-    erewrite (@program_lsim_init_mem_match Language_RTL Language_RTL); try apply transf_efT_sigT; eauto.
-    unfold ge0 in *. erewrite symbols_preserved; eauto. 
-    destruct Hfsim as [_ Hmain]. unfold fundef in *. simpl in *. rewrite <- Hmain. auto.
-    rewrite <- H3. eapply sig_preserved; eauto. 
+    exploit (init_mem_transf_partial TRANSF); eauto.
+    rewrite symbols_preserved. 
+    inv TRANSF. unfold fundef in *. simpl in *. rewrite <- Hmain. unfold ge, ge0 in *. congruence.
+    rewrite <- H3. eapply sig_function_translated; eauto. 
   econstructor; eauto. 
   instantiate (1 := Mem.flat_inj (Mem.nextblock m0)). 
   apply match_stacks_nil with (Mem.nextblock m0).
@@ -926,263 +1309,22 @@ Proof.
 Qed.
 
 Lemma transf_final_states:
-  forall F st1 st2 r, 
-  match_states F st1 st2 -> final_state st1 r -> final_state st2 r.
+  forall st1 st2 r, 
+  match_states st1 st2 -> final_state st1 r -> final_state st2 r.
 Proof.
   intros. inv H0. inv H.
   exploit match_stacks_empty; eauto. intros EQ; subst. inv VINJ. constructor.
   exploit match_stacks_inside_empty; eauto. intros [A B]. congruence. 
 Qed.
 
-Inductive match_states_ext F st tst: Prop :=
-| match_states_ext_intro
-    (Hsrc: sound_state_ext fprog st)
-    (Htgt: sound_state_ext ftprog tst)
-    (Hmatch: match_states F st tst)
-.
-
-End FUTURE.
-
-(* memory relation *)
-
-Inductive mrelT_sem (mrel:meminj) (fprog ftprog:program) (i:WF.t) (s1 s2:state): Prop :=
-| mrelT_sem_intro
-    (MEASURE: i = WF.from_nat (measure s1))
-    (Hsrc: sound_state_ext fprog s1)
-    (Htgt: sound_state_ext ftprog s2)
-    (MS: match_states fprog mrel s1 s2 \/ match_call fprog ftprog mrel s1 s2)
-.
-
-Definition mrelT_ops: mrelT_opsT Language_ext_RTL Language_ext_RTL meminj :=
-  mkmrelT_opsT
-    Language_ext_RTL Language_ext_RTL
-    mrelT_sem
-    (fun mrel v1 v2 => val_inject mrel v1 v2)
-    (fun _ _ => True)
-    (fun _ _ => True).
-
-Lemma mrelT_ops_val_inject_list mrel v1 v2:
-  val_list_inject mrel v1 v2 <-> list_forall2 (mrelT_ops.(sem_value) mrel) v1 v2.
+Theorem transf_program_correct:
+  forward_simulation (semantics prog) (semantics tprog).
 Proof.
-  revert v2.
-  induction v1; intros; constructor; intro H; inv H; constructor; auto.
-  - apply IHv1. auto.
-  - apply IHv1. auto.
-Qed.
-
-Program Definition mrelT_props:
-  @mrelT_propsT Language_ext_RTL Language_ext_RTL
-                transf_sigT transf_efT transf_vT _ mrelT_ops :=
-  mkmrelT_propsT _ _ _ _ _ _ _.
-Next Obligation. repeat constructor. Qed.
-Next Obligation. repeat constructor. Qed.
-Next Obligation. inv H. auto. Qed.
-Next Obligation.
-  apply initial_state_RTL_equiv in H1. apply initial_state_RTL_equiv in H2.
-  exploit transf_initial_states; eauto. intros [F [st2 [Hst2 Hmatch]]].
-  exists F. eexists. constructor; eauto.
-  { apply sound_initial. auto. }
-  { apply sound_initial. auto. }
-  right.
-  inv H2. inv Hst2. unfold ge, ge0 in *.
-  rewrite H in H2. inv H2. rewrite H0 in H5. inv H5. rewrite H3 in H6. inv H6.
-  auto.
-Qed.
-Next Obligation.
-  simpl in *. apply (mrelT_ops_val_inject_list mrel args1 args2) in Hargs.
-  destruct fd1; inv Hfd1. destruct fd2; inv Hfd2.
-  inv Hs0. inv Hmrel. destruct MS as [MS|MS]; inv MS.
-
-  (* external function *)
-  exploit match_stacks_globalenvs; eauto. intros [bound MG].
-  exploit external_call_mem_inject; eauto.
-    eapply match_globalenvs_preserves_globals; eauto.
-    intros [F1 [v1 [m1'' [A [B [C [D [E [J K]]]]]]]]].
-  eexists. eexists. eexists. eexists. eexists. exists F1. eexists.
-  repeat (split; [eauto; fail|]). split.
-  - econstructor. eapply external_call_symbols_preserved; eauto.
-    + eapply symbols_preserved. apply Hp.
-    + eapply varinfo_preserved. apply Hp.
-  - split; auto.
-    constructor; eauto.
-    { eapply sound_past_step; eauto. econstructor. eauto. }
-    { eapply sound_past_step; eauto. econstructor.
-      eapply external_call_symbols_preserved; eauto.
-      + eapply symbols_preserved. apply Hp.
-      + eapply varinfo_preserved. apply Hp.
-    }
-    left. constructor; auto.
-    eapply match_stacks_bound with (Mem.nextblock m2).
-    eapply match_stacks_extcall with (F1 := mrel) (F2 := F1) (m1 := m1) (m1' := m2); eauto.
-    intros; eapply external_call_max_perm; eauto.
-    intros; eapply external_call_max_perm; eauto.
-    xomega.
-    eapply external_call_nextblock; eauto.
-Qed.
-
-Section STATE_LSIM.
-  
-Variable (fprog ftprog:program).
-Hypothesis (Hfsim: @program_weak_lsim Language_RTL Language_RTL transf_sigT transf_efT transf_vT
-                                      fprog ftprog).
-
-Hypothesis (Hfprog: program_linkeq Language_RTL prog fprog).
-Hypothesis (Hftprog: program_linkeq Language_RTL tprog ftprog).
-
-Lemma match_states_state_lsim es es' (eF F:meminj) s1 s1'
-      (MS: match_states_ext fprog ftprog F s1 s1'):
-  @state_lsim Language_ext_RTL Language_ext_RTL transf_sigT transf_efT _
-              mrelT_ops fprog ftprog es es' eF F (WF.from_nat (measure s1)) s1 s1'.
-Proof.
-  revert F s1 s1' MS. pcofix CIH. intros F s1 s1' MS. pfold.
-  inv MS. destruct (classic (exists r, final_state s1 r)).
-  { destruct H as [rval Hrval]. eapply _state_lsim_term; eauto.
-    - apply final_state_RTL_equiv. eauto.
-    - apply final_state_RTL_equiv. eapply transf_final_states; eauto.
-  }
-  constructor; auto.
-  { repeat intro. apply H. exists r0. apply final_state_RTL_equiv. auto. }
-  intros. exploit step_simulation; eauto. simpl.
-  intros [[F' [s2' [Hs2' Hmatch']]]|[mrel2 [Hmrel2 [Hevt Hmatch']]]].
-  - eexists. exists s2'. exists F'.
-    split; [auto|]. split; [auto|]. split; [constructor; auto|].
-    { eapply sound_past_step; eauto. }
-    { eapply sound_past_plus; eauto. }
-    destruct Hmatch' as [Hmatch'|Hmatch'].
-    + constructor. right. apply CIH; auto. constructor; auto.
-      * eapply sound_past_step; eauto.
-      * eapply sound_past_plus; eauto.
-    + inversion Hmatch'. subst. eapply _state_lsim_or_csim_csim; eauto.
-      { apply mrelT_ops_val_inject_list. auto. }
-      { constructor; auto.
-        - eapply sound_past_step; eauto.
-        - eapply sound_past_plus; eauto.
-      }
-      intros. right. inv Hst2_mem. apply CIH.
-      constructor; auto. econstructor; eauto.
-      destruct MS0 as [MS0|MS0]; inv MS0; auto. 
-      destruct MS0 as [MS0|MS0]; inv MS0; auto. 
-  - subst. eexists. exists s1'. exists mrel2.
-    split.
-    { right. split; [apply star_refl|]. constructor. eauto. }
-    split; [auto|]. split; [constructor; auto|].
-    { eapply sound_past_step; eauto. }
-    destruct Hmatch' as [Hmatch'|Hmatch'].
-    + constructor. right. apply CIH; auto. constructor; auto.
-      eapply sound_past_step; eauto.
-    + inversion Hmatch'. subst. eapply _state_lsim_or_csim_csim; eauto.
-      { apply mrelT_ops_val_inject_list. auto. }
-      { constructor; auto.
-        eapply sound_past_step; eauto.
-      }
-      intros. right. inv Hst2_mem. apply CIH.
-      constructor; auto. econstructor; eauto.
-      destruct MS0 as [MS0|MS0]; inv MS0; auto. 
-      destruct MS0 as [MS0|MS0]; inv MS0; auto. 
-Qed.
-
-Lemma transf_function_lsim
-      fenv (FENV: PTree_le fenv (funenv_program fprog))
-      f f' (Hfd: Inlining.transf_function fenv f = OK f'):
-  @function_lsim Language_ext_RTL Language_ext_RTL transf_sigT transf_efT _
-                 mrelT_ops fprog ftprog f f'.
-Proof.
-  constructor. repeat intro. inv Hmrel_entry.
-  destruct MS as [MS|MS]; inv MS.
-  pfold. constructor; auto.
-  { intros ? Hfinal. apply final_state_RTL_equiv in Hfinal. inv Hfinal. }
-  intros. destruct fd_src; inv Hfd_src. destruct fd_tgt; inv Hfd_tgt. inversion Hst2_src. subst.
-
-  (* internal function, not inlined *)
-  assert (TR: tr_function fenv f f'). 
-    eapply transf_function_spec; eauto. 
-  inversion TR; subst.
-  exploit Mem.alloc_parallel_inject. eauto. eauto. apply Zle_refl. 
-    instantiate (1 := fn_stacksize f'). inv H. xomega. 
-  intros [F' [m1' [sp' [A [B [C [D E]]]]]]].
-  eexists. eexists. eexists. split.
-  left. eapply plus_one. eapply exec_function_internal; eauto.
-  instantiate (2 := F'). split; [simpl; auto|].
-  cut (match_states fprog F'
-                    (State es_src f (Vptr stk Int.zero) (fn_entrypoint f)
-                           (init_regs args_src (fn_params f)) m')
-                    (State es_tgt f' (Vptr sp' Int.zero) (fn_entrypoint f')
-                           (init_regs args_tgt (fn_params f')) m1')).
-  { intro MS. split; [constructor; eauto|].
-    { eapply sound_past_step; eauto. }
-    { eapply sound_past_step; eauto. constructor; auto. }
-    constructor. left. apply match_states_state_lsim. constructor; auto.
-    - eapply sound_past_step; eauto.
-    - eapply sound_past_step; eauto. constructor; auto.
-  }
-  rewrite H4. econstructor.
-  apply match_stacks_inside_base.
-  assert (SP: sp' = Mem.nextblock mem_entry_tgt) by (eapply Mem.alloc_result; eauto).
-  rewrite <- SP in MS0.
-  eapply match_stacks_invariant; eauto.
-    intros. destruct (eq_block b1 stk).
-    subst b1. rewrite D in H7; inv H7. subst b2. eelim Plt_strict; eauto.
-    rewrite E in H7; auto.
-    intros. exploit Mem.perm_alloc_inv. eexact H5. eauto.
-    destruct (eq_block b1 stk); intros; auto.
-    subst b1. rewrite D in H7; inv H7. subst b2. eelim Plt_strict; eauto.
-    intros. eapply Mem.perm_alloc_1; eauto.
-    intros. exploit Mem.perm_alloc_inv. eexact A. eauto.
-    rewrite dec_eq_false; auto.
-  auto. auto. auto. eauto. auto.
-  rewrite H3. apply agree_regs_init_regs. eauto. auto. inv H; auto. congruence. auto.
-  eapply Mem.valid_new_block; eauto.
-  red; intros. split.
-  eapply Mem.perm_alloc_2; eauto. inv H; xomega.
-  intros; red; intros. exploit Mem.perm_alloc_inv. eexact H5. eauto.
-  destruct (eq_block b stk); intros.
-  subst. rewrite D in H8; inv H8. inv H; xomega.
-  rewrite E in H8; auto. eelim Mem.fresh_block_alloc. eexact A. eapply Mem.mi_mappedblocks; eauto.
-  auto.
-  intros. exploit Mem.perm_alloc_inv; eauto. rewrite dec_eq_true. omega.
-Qed.
-
-End STATE_LSIM.
-
-Lemma Inlining_program_lsim:
-  @program_lsim Language_RTL Language_RTL transf_sigT transf_efT transf_vT
-                (@function_lsim Language_ext_RTL Language_ext_RTL transf_sigT transf_efT _ mrelT_ops)
-                prog tprog.
-Proof.
-  generalize transf_function_lsim.
-  destruct prog as [defs main]. simpl in *. simpl in *.
-  unfold transf_program, transform_partial_program, transform_partial_program2 in TRANSF.
-  Errors.monadInv TRANSF. rename x into tdefs.
-  simpl in *. intro Hlsim. constructor; simpl; auto.
-  revert Hlsim EQ.
-  generalize tdefs at 2 as ftdefs.
-  generalize defs at 1 3 as fdefs.
-  revert defs tdefs.
-  induction defs; simpl; intros tdefs fdefs ftdefs Hlsim Hglobdefs; inv Hglobdefs; try constructor.
-  destruct a. destruct g.
-  - match goal with
-      | [H: match ?tf with | OK _ => _ | Error _ => _ end = _ |- _] => destruct tf eqn:Htf; inv H
-    end.
-    Errors.monadInv H1. constructor; simpl in *; try apply IHdefs; auto.
-    split; auto. apply (@globdef_lsim_fun Language_RTL Language_RTL).
-    destruct f; simpl in *.
-    + Errors.monadInv Htf. constructor; simpl; intros.
-      unfold Inlining.transf_function in EQ0.
-      repeat match goal with
-               | [H: context[let 'R _ _ _ := ?r:res in _] |- _] => destruct r eqn:Hr
-               | [H: context[zlt ?a ?b] |- _] => destruct (zlt a b); inv H
-             end.
-      simpl. split; auto.
-      repeat intro. exploit Hlsim; eauto.
-      { apply program_linkeq_fenv_le. eauto. }
-      unfold Inlining.transf_function.
-      rewrite Hr. rewrite zlt_true; auto.
-    + inv Htf.
-      eapply globfun_lsim_intro; eauto; simpl; auto.
-  - Errors.monadInv H0.
-    constructor; simpl in *; try apply IHdefs; auto.
-    split; auto. apply (@globdef_lsim_var Language_RTL Language_RTL).
-    repeat constructor.
+  eapply forward_simulation_star.
+  eexact symbols_preserved.
+  eexact transf_initial_states.
+  eexact transf_final_states.
+  eexact step_simulation. 
 Qed.
 
 End INLINING.
