sepcomp/common/Language.v
@@ -1,9 +1,9 @@
 Require Import RelationClasses.
 Require String.
-Require Import Coqlib Coqlib_linker.
-Require Import Maps Maps_linker.
+Require Import Coqlib Coqlib_sepcomp.
+Require Import Maps Maps_sepcomp.
 Require Import Integers Floats Values AST Globalenvs.
-Require Import Errors Behaviors Compiler Smallstep Smallstep_linker.
+Require Import Errors Behaviors Compiler Smallstep Smallstep_sepcomp.
 Require Import Memory.
 
 Set Implicit Arguments.
