sepcomp/common/LinkerProp.v
@@ -1,7 +1,7 @@
 Require Import RelationClasses.
 Require String.
-Require Import Coqlib Coqlib_linker.
-Require Import Maps Maps_linker.
+Require Import Coqlib Coqlib_sepcomp.
+Require Import Maps Maps_sepcomp.
 Require Import Integers Floats Values AST Globalenvs.
 Require Import Language Linker.
 Require Import Errors.
