sepcomp/build.sh
@@ -1,8 +1,7 @@
 #!/usr/bin/env bash
-make -f sepcomp/Makefile depend
-make -f sepcomp/Makefile -j $1 proof
-make -f sepcomp/Makefile extraction
-make -f sepcomp/Makefile ccomp
-make -f sepcomp/Makefile runtime
+make -f sepcomp/Makefile depend &&
+make -f sepcomp/Makefile -j $1 proof &&
+make -f sepcomp/Makefile extraction &&
+make -f sepcomp/Makefile ccomp &&
+make -f sepcomp/Makefile runtime &&
 make -f sepcomp/Makefile cchecklink
-
